# Jugs of Water

First, fill the 3-quart jug. Then pour the 3-quart jug into the 5-quart jug.
Fill the 3-quart jug again and use it to fill the 5-quart jug to the brim. This
will leave 1 quart of water in the 3-quart jug and 5 quarts in the 5-quart jug.
Empty the 5-quart jug, and then pour the 1 quart from the 3-quart jug into it.
Refill the 3-quart jug to the brim from the source, and then pour those
additional 3 quarts into the 5-quart jug. The 5-quart jug will then have 4
quarts of water.

Let $(a, b)$ represent $a$ quarts of water in the 5-quart jug and $b$ quarts in
the 3-quart jug. We can then represent our solution as the following sequence:

$$
\begin{align*}
(0, 0) \to (0, 3) \to (3,0) \to (3, 3) \to (5, 1) \to (0, 1) \to (1, 0)
\to (1, 3) \to (4, 0).
\end{align*}
$$
